\documentclass[UTF8,9pt]{ctexart}
\usepackage{../template/Notes/notes}
\title{Theoretical Mechanics}
\renewcommand\arraystretch{1.5}
\begin{document}
    \maketitle

    \section{è´¨ç‚¹åŠ›å­¦}
        æåæ ‡ï¼š
        $$
        \begin{array}{rl}
            \bm{v}=&\dot{r}\bm{i}_{r}+r\dot{\theta}\bm{j}_{\theta}   \\
            \bm{a}=&\left(\ddot{r}-r\dot{\theta}^2\right)\bm{i}_{r}+\dfrac{1}{r}\dfrac{\dif}{\dif t}\left(r^2\dot{\theta}\right)\bm{j}_{\theta}\\
            =&(a_r-r\omega^2)\bm{i}_r+\dfrac{1}{r}\dfrac{\dif}{\dif t}\left(r^2\omega\right)\bm{j}_{\theta}
        \end{array}
        $$ 
        è‡ªç„¶åæ ‡ç³»ï¼š
        $$
        \begin{array}{rl} 
            a_t=&\dfrac{\dif v}{\dif t}  \\
            a_n=&\dfrac{v^2}{\rho}       \\
            \dfrac{\mathrm{d}}{\mathrm{d}t}=&\dfrac{\mathrm{d}'}{\mathrm{d}t}+\omega\times 
        \end{array}
        $$
        æ›²ç‡ï¼š
        $$\dfrac{1}{\rho}=\dfrac{|y''|}{\left(1+y'^2\right)^{3/2}}=-\dfrac{\dif s}{\dif \theta}$$
        æœ‰å¿ƒåŠ›åœºèƒ½é‡å…³ç³»ï¼š
        $$\dfrac{1}{2}m\left(\dot{r}^2+r^2\dot{\theta}^2\right)+V(r)=E$$
        æœ‰å¿ƒåŠ›åœºæ¯”è€å…¬å¼ï¼š
        $$h^2u^2\left(\dfrac{\dif^2u}{\dif \theta^2}+u\right)=-\dfrac{F}{m}\ \left( \begin{array}{ll}
            h=&r^2\dot{\theta}\\
            u=&\dfrac{1}{r}
        \end{array}\right) $$
        æ˜Ÿä½“è½¨é“æ–¹ç¨‹ï¼š
        $$\begin{array}{rl}
            r=&\dfrac{h^2/k^2}{1+\sqrt{1+2h^2E/(k^4m)}\left[\cos(\theta-\theta_0)\right]}, \\
            e=&\sqrt{1+\dfrac{2E}{m}(h/k^2)^2}
        \end{array}$$
        æ›²ç‡åŠå¾„ï¼š
        $$\rho=\dfrac{\left[1+y'^2\right]^{3/2}}{|y''|}=\frac{v^3}{|\bm{v}\times\bm{a}|}$$
        ä½åŠ›å®šç†ï¼š
        $$V=ar^{n+1} \Leftimplies \bar{T}=\frac{1}{2}(n+1)\bar{V}$$
    \section{åˆšä½“åŠ›å­¦}
        åŠ¨é‡çŸ©ï¼š
        $$\bm{J}=\sum_{i=1}^n\left[\bm{\omega}r_i^2-\bm{r}_i(\bm{\omega\cdot r}_i)\right]$$
        $$J_x=I_{xx}\omega_x-I_{xy}\omega_y-I_{xz}\omega_z$$
        è½¬åŠ¨æƒ¯é‡ï¼š
        $$I_{xx}=\sum_{i=1}^nm_i(y_i^2+z_i^2)=\int(y_i^2+z_i^2)\,\dif m$$
        $$I_{yz}=\sum_{i=1}^nm_iy_iz_i=\int y_iz_i\,\dif m$$
        $$I=\sum_{i,j,k=x_i,\,\alpha_i}\left(  I_{ii}\alpha_i^2-2I_{jk}\alpha_j\alpha_k\right),\  \alpha_i\text{ä¸ºæ–¹å‘ä½™å¼¦}$$
        $$I=\sum m_i\rho_i^2$$
        è½¬åŠ¨åŠ¨èƒ½ï¼š
        $$T=\frac{1}{2}\sum_{i,j,k=x_i}\left(I_{ii}\omega_i^2-2I_{jk}\omega_j\omega_k\right)=\frac{1}{2}I\omega^2$$
        $\qquad$é€‰å–æƒ¯é‡ä¸»è½´ä¸ºåæ ‡è½´æ—¶ï¼š
        $$T=\frac{1}{2}\sum_{i,j,k=x_i}I_{i}\omega_i^2$$
        $\qquad$å¹³é¢å¹³è¡Œè¿åŠ¨ï¼š
        $$T=\frac{1}{2}mv^2_c+\frac{1}{2}I_{zz}\omega^2$$
        æ»šåŠ¨æ‘©æ“¦ï¼š
        $$M=Nk$$
        å˜è´¨é‡ç‰©ä½“ï¼š
        $$F=\dift{mv}-\dift{m} u$$
    \section{åˆ†æåŠ›å­¦}
        å¹¿ä¹‰åŠ›ï¼š
        $$Q_\alpha=\sum_{i=1}^n F_i\pari{r_i}{q_\alpha}$$
        Lagrange{\fontspec{Segoe UI Emoji}ğŸŠ}\,æ³•
        $$\left\{\begin{array}{rl}
            F_{ix}+\sum_{\beta=1}^k\lambda_\beta\pari{f_\beta}{x_i}&=0\\
            F_{iy}+\sum_{\beta=1}^k\lambda_\beta\pari{f_\beta}{y_i}&=0\\
            F_{iz}+\sum_{\beta=1}^k\lambda_\beta\pari{f_\beta}{z_i}&=0\\
            \sum_{\beta=1}^kf_\beta(x,y,z)&=0
        \end{array}\right.$$
        å…¶ä¸­ï¼Œ$\bm{R}=\lambda\nabla f$\\
        Lagrangeæ–¹ç¨‹ï¼š
        $$\dift{}\left(\frac{\partial T}{\partial \dot{q_{\alpha}}}\right)-\frac{\partial T}{\partial q_{\alpha}}=Q_{\alpha}$$
        $$\dift{}\left(\frac{\partial L}{\partial \dot{q_{\alpha}}}\right)-\frac{\partial L}{\partial q_{\alpha}}=0$$
        å“ˆå¯†é¡¿æ–¹ç¨‹ï¼š  
        $$\left\{\begin{array}{rr}
            \dot{q}_{\alpha}=&\dfrac{\partial H}{\partial p_{\alpha}} \\
            \dot{p}_{\alpha}=&-\dfrac{\partial H}{\partial q_{\alpha}}
        \end{array}\right.$$
\end{document}